-

PermutSeq.v
@@ -3409,20 +3409,31 @@ apply Nat.mod_upper_bound.
 apply fact_neq_0.
 Qed.
 
-(*
-Definition permut_inv n (σ : vector nat) :=
-  mk_vect n (permut_fun_inv (vect_el σ) n).
-*)
+Definition permut_inv (n : nat) (σ : vector nat) :=
+  mk_vect (map (permut_fun_inv (vect_nat_el σ) n) (seq 0 n)).
 
-(*
-Theorem permut_inv_is_permut : ∀ n (σ : vector n nat),
-  is_permut_vect σ
-  → is_permut_vect (permut_inv σ).
+Theorem permut_inv_is_permut : ∀ n (σ : vector nat),
+  is_permut_vect n σ
+  → is_permut_vect n (permut_inv n σ).
 Proof.
+intros * Hperm.
+unfold permut_inv.
+unfold is_permut_vect.
+Check permut_fun_inv_is_permut.
+Print vect_nat_el.
+...
+unfold is_permut_vect.
+unfold permut_inv.
+unfold vect_nat_el.
+cbn.
+Check permut_fun_inv_is_permut.
+Print permut_fun_inv.
+...
 intros * Hperm.
 now apply permut_fun_inv_is_permut.
 Qed.
-*)
+
+...
 
 Theorem sym_gr_inv_upper_bound : ∀ n k j,
   k < fact n
